\documentclass{article}
\usepackage{tikz}
\usepackage{float}
\usepackage{enumerate}
\usepackage{amsmath}
\usepackage{bm}
\usepackage{indentfirst}
\usepackage{siunitx}
\usepackage[utf8]{inputenc}
\usepackage{graphicx}
\graphicspath{ {Images/} }
\usepackage{float}
\usepackage{mhchem}
\usepackage{chemfig}
\allowdisplaybreaks

\title{ 6.042 Session 4 }
\author{ Robert Durfee }
\date{ February 14, 2018 }

\begin{document}

\maketitle

\section*{Problem 1}

The full disjunctive normal form for the formula:
\begin{align*}
  (A \land B \land C \land D) &\lor
  (A \land B \land \overline{C} \land D)\ \lor \\
  (A \land \overline{B} \land C \land D) &\lor
  (A \land \overline{B} \land C \land \overline{D})\ \lor \\
  (A \land \overline{B} \land \overline{C} \land D) &\lor
  (A \land \overline{B} \land \overline{C} \land \overline{D})\ \lor \\
  (\overline{A} \land B \land C \land D) &\lor
  (\overline{A} \land B \land \overline{C} \land D)\ \lor \\
  (\overline{A} \land \overline{B} \land \overline{C} \land D) &\lor
  (\overline{A} \land \overline{B} \land \overline{C} \land \overline{D})
\end{align*}

The full conjunctive normal form for the formula:
\begin{align*}
  (\overline{A} \lor \overline{B} \lor \overline{C} \lor D) &\land
  (\overline{A} \lor \overline{B} \lor C \lor D)\ \land \\
  (A \lor \overline{B} \lor \overline{C} \lor D) &\land
  (A \lor \overline{B} \lor C \lor D)\ \land \\
  (A \lor B \lor \overline{C} \lor \overline{D}) &\land
  (A \lor B \lor \overline{C} \lor D)
\end{align*}

\section*{Problem 2}

$$ A \oplus B \oplus C $$
$$ (A \oplus B) \oplus C $$
$$ ((A \land \overline{B}) \lor (\overline{A} \land B)) \oplus C $$
$$ (((A \land \overline{B}) \lor (\overline{A} \land B)) \land \overline{C})
\lor \overline{(((A \land \overline{B}) \lor (\overline{A} \land B))} \land C) $$
$$ (((A \land \overline{B}) \lor (\overline{A} \land B)) \land \overline{C})
\lor ((\overline{(A \land \overline{B})} \land \overline{(\overline{A} \land B)}) \land C)  $$
$$ (((A \land \overline{B}) \lor (\overline{A} \land B)) \land \overline{C})
\lor (((\overline{A} \lor B) \land (A \lor \overline{B})) \land C) $$
$$ (A \land \overline{B} \land \overline{C}) \lor (\overline{A} \land B \land
\overline{C}) \lor (((\overline{A} \lor B) \land (A \lor \overline{B})) \land C) $$
$$ (A \land \overline{B} \land \overline{C}) \lor (\overline{A} \land B \land
\overline{C}) \lor (((\overline{A} \land A) \lor (\overline{A} \land
\overline{B}) \lor (B \land A) \lor (B \land \overline{B})) \land C) $$
$$ (A \land \overline{B} \land \overline{C}) \lor (\overline{A} \land B \land
\overline{C}) \lor ((F \lor (\overline{A} \land \overline{B}) \lor (B \land A)
\lor F) \land C)$$
$$ (A \land \overline{B} \land \overline{C}) \lor (\overline{A} \land B \land
\overline{C}) \lor (((\overline{A} \land \overline{B}) \lor (B \land A)) \land C) $$
$$ (A \land \overline{B} \land \overline{C}) \lor (\overline{A} \land B \land
\overline{C}) \lor (\overline{A} \land \overline{B} \land C) \lor (A \land B
\land C) $$

\section*{Problem 3}

\begin{enumerate}[a.]
  \item In order for the statement to be satisfiable, the individual components
    must be satisfiable. Therefore, a logical and of all the parts and the whole
    statement will be satisfiable if and only if the whole is satisfiable.
\end{enumerate}

\end{document}

